Linearized InsertImpl with iffy returns work around

Impl/InsertImpl.i.dfy
@@ -37,84 +37,87 @@ module InsertImpl {
   import opened NodeImpl
   import opened BoundedPivotsLib
 
-  method InsertKeyValue(s: ImplVariables, key: Key, value: Value)
+  method InsertKeyValue(linear inout s: ImplVariables, key: Key, value: Value)
   returns (success: bool)
-  requires Inv(s)
-  requires s.ready
-  requires BT.G.Root() in s.cache.I()
-  requires |s.ephemeralIndirectionTable.I().graph| <= IT.MaxSize() - 1
-  requires BoundedKey(s.cache.I()[BT.G.Root()].pivotTable, key)
-  modifies s.Repr()
-  ensures WellUpdated(s)
-  ensures (s.I(), success) == InsertModel.InsertKeyValue(old(s.I()), key, value)
+  requires old_s.Inv()
+  requires old_s.ready
+  requires BT.G.Root() in old_s.cache.I()
+  requires |old_s.ephemeralIndirectionTable.I().graph| <= IT.MaxSize() - 1
+  requires BoundedKey(old_s.cache.I()[BT.G.Root()].pivotTable, key)
+  ensures s.W()
+  ensures (s.I(), success) == InsertModel.InsertKeyValue(old_s.I(), key, value)
   {
     InsertModel.reveal_InsertKeyValue();
 
     BookkeepingModel.lemmaChildrenConditionsOfNode(s.I(), BT.G.Root());
+    success := true;
 
-    if s.frozenIndirectionTable != null {
-      var b := s.frozenIndirectionTable.HasEmptyLoc(BT.G.Root());
+    if s.frozenIndirectionTable.lSome? {
+      var b := s.frozenIndirectionTable.value.HasEmptyLoc(BT.G.Root());
       if b {
         success := false;
         print "giving up; can't dirty root because frozen isn't written";
-        return;
       }
     }
 
-    var msg := ValueMessage.Define(value);
-    s.cache.InsertKeyValue(BT.G.Root(), key, msg);
+    if (success) {
+      var msg := ValueMessage.Define(value);
+      inout s.cache.InsertKeyValue(BT.G.Root(), key, msg);
 
-    writeBookkeepingNoSuccsUpdate(s, BT.G.Root());
-
-    success := true;
+      writeBookkeepingNoSuccsUpdate(inout s, BT.G.Root());
+    }
   }
 
-  method insert(s: ImplVariables, io: DiskIOHandler, key: Key, value: Value)
+  //TODO Check to see if casing on success is OK
+  //     Before it returned but cant do that with linear
+  method insert(linear inout s: ImplVariables, io: DiskIOHandler, key: Key, value: Value)
   returns (success: bool)
   requires io.initialized()
-  requires Inv(s)
-  requires io !in s.Repr()
-  requires s.ready
-  modifies s.Repr()
+  requires old_s.Inv()
+  requires old_s.ready
   modifies io
-  ensures WellUpdated(s)
-  ensures InsertModel.insert(old(s.I()), old(IIO(io)), key, value, s.I(), success, IIO(io))
+  ensures s.W()
+  ensures InsertModel.insert(old_s.I(), old(IIO(io)), key, value, s.I(), success, IIO(io))
   {
     InsertModel.reveal_insert();
+    success := true;
 
     var indirectionTableSize := s.ephemeralIndirectionTable.GetSize();
     if (!(indirectionTableSize <= IT.MaxSizeUint64() - 3)) {
       success := false;
-      return;
     }
 
-    var rootLookup := s.cache.InCache(BT.G.Root());
-    if !rootLookup {
-      if TotalCacheSize(s) <= MaxCacheSizeUint64() - 1 {
-        PageInNodeReq(s, io, BT.G.Root());
+    if (success){
+      var rootLookup := s.cache.InCache(BT.G.Root());
+      if !rootLookup {
+        if s.TotalCacheSize() <= MaxCacheSizeUint64() - 1 {
+          PageInNodeReq(inout s, io, BT.G.Root());
+          success := false;
+        } else {
+          print "insert: root not in cache, but cache is full\n";
+          success := false;
+        }
+      }
+    }
+
+    if (success) {
+      var pivots, _ := s.cache.GetNodeInfo(BT.G.Root());
+      var bounded := ComputeBoundedKey(pivots, key);
+      if !bounded {
         success := false;
+        print "giving up; can't insert key at root because root is incorrects";
+      }
+    }
+
+    if (success) {
+      var weightSeq := s.cache.NodeBucketsWeight(BT.G.Root());
+      if WeightKeyUint64(key) + WeightMessageUint64(ValueMessage.Define(value)) + weightSeq
+        <= MaxTotalBucketWeightUint64() {
+          success := InsertKeyValue(inout s, key, value);
       } else {
-        print "insert: root not in cache, but cache is full\n";
+        runFlushPolicy(inout s, io);
         success := false;
       }
-      return;
-    }
- 
-    var pivots, _ := s.cache.GetNodeInfo(BT.G.Root());
-    var bounded := ComputeBoundedKey(pivots, key);
-    if !bounded {
-      success := false;
-      print "giving up; can't insert key at root because root is incorrects";
-      return;
-    }
-
-    var weightSeq := s.cache.NodeBucketsWeight(BT.G.Root());
-    if WeightKeyUint64(key) + WeightMessageUint64(ValueMessage.Define(value)) + weightSeq
-        <= MaxTotalBucketWeightUint64() {
-      success := InsertKeyValue(s, key, value);
-    } else {
-      runFlushPolicy(s, io);
-      success := false;
     }
   }
 }
